smtlink/SMT-extract.lisp
@@ -1,0 +1,14 @@
+;; SMT-extract extracts the declarations, hypotheses and conclusion from a SMT formula in ACL2.
+;; A typical SMT formula is in below format:
+;; (implies (and <decl-list>
+;;               <hypo-list>)
+;;          <concl-list>)
+
+;; SMT-extract
+(defun SMT-extract (term)
+  "extract decl-list, hypo-list and concl from a ACL2 term"
+  (let ((decl-list (cadr (cadr term)))
+	(hypo-list (caddr (cadr term)))
+	(concl-list (caddr term)))
+    (prog2$ (cw "extract: ~q0 ~q1 ~q2" decl-list hypo-list concl-list)
+	    (mv decl-list hypo-list concl-list))))
