smtlink/helper.lisp
@@ -35,3 +35,62 @@
 (defthm delete-must-reduce
     (implies (exist a listx)
 	     (< (len (my-delete listx a)) (len listx))))
+
+;; append-and
+(defun append-and (listx listy)
+  "append-and: append two and lists together in the underneath representation"
+  (if (endp listy)
+      listx
+      (list 'if listx listy 'nil)))
+
+;; assoc-no-repeat
+(defun assoc-no-repeat (assoc-list)
+  "assoc-no-repeat: check if an associate list has repeated keys"
+  (if (endp assoc-list)
+      t
+      (if (equal (assoc (caar assoc-list) (cdr assoc-list)) nil)
+	  (assoc-no-repeat (cdr assoc-list))
+	  nil)))
+
+;; invert-assoc
+(defun invert-assoc (assoc-list)
+  "invert-assoc: invert the key and value pairs in an associate list"
+  (if (endp assoc-list)
+      nil
+      (cons (list (cadr (car assoc-list)) (car (car assoc-list)))
+	   (invert-assoc (cdr assoc-list)))))
+
+;; create-assoc-helper
+ (defun create-assoc-helper (list-keys list-values)
+   (if (endp list-keys)
+       nil
+       (cons (list (car list-keys) (car list-values))
+	     (create-assoc-helper (cdr list-keys) (cdr list-values)))))
+
+;; create-assoc
+(defun create-assoc (list-keys list-values)
+  "create-assoc: combines two lists together to form an associate list"
+  (if (equal (len list-keys) (len list-values))
+      (create-assoc-helper list-keys list-values)
+      (cw "Error(helper): list-keys and list-values should be of the same len.")))
+
+;; replace-lambda-params
+ (defun replace-lambda-params (expr lambda-params-mapping)
+   "replace-lambda-params: replace params in the expression using the mapping"
+   (if (atom expr)
+       (let ((res (assoc expr lambda-params-mapping)))
+	 (if (equal res nil)
+	     expr
+	     (cadr res)))
+       (cons (replace-lambda-params (car expr) lambda-params-mapping)
+	     (replace-lambda-params (cdr expr) lambda-params-mapping))))
+
+;; assoc-lambda
+(defun assoc-lambda (expr lambda-params-mapping assoc-list)
+  "assoc-lambda: replacing params in expression using lambda-params-mapping \
+and check if the resulting term exist in assoc-list keys. Return the resulting \
+pair from assoc-list."
+  (b* ((new-expr (replace-lambda-params expr lambda-params-mapping))
+       (final-res (assoc new-expr assoc-list)))
+      final-res)
+  )
